introduce MonadAttach and instances
wip

wip

fix iterator definitions except ranges

oof: fixed range errors

Oof

revert :(

begin and discard the combinator approach

wip

it builds

more instances

wip: WeaklyLawfulMonadAttach

use WeaklyLawfulMonadAttach instead of LawfulMonadAttach

add trivial instances for CPS monads

add docstrings and instances

add missing filterMap lemmas

update docstrings

fix tests

src/Init/Data/Iterators/Combinators/Monadic/FilterMap.lean
@@ -123,7 +123,7 @@ returned `Option` value.
 def IterM.filterMapWithPostcondition {α β γ : Type w} {m : Type w → Type w'} {n : Type w → Type w''}
     [MonadLiftT m n] [Iterator α m β] (f : β → PostconditionT n (Option γ))
     (it : IterM (α := α) m β) : IterM (α := FilterMap α m n (fun ⦃_⦄ => monadLift) f) n γ :=
-  IterM.InternalCombinators.filterMap (fun ⦃_⦄ => monadLift) f it
+  IterM.InternalCombinators.filterMap (n := n) (fun ⦃_⦄ => monadLift) f it
 
 namespace Iterators.Types
 
@@ -382,12 +382,8 @@ it.filterMapM     ---a'-----c'-------⊥
 For certain mapping functions `f`, the resulting iterator will be finite (or productive) even though
 no `Finite` (or `Productive`) instance is provided. For example, if `f` never returns `none`, then
 this combinator will preserve productiveness. If `f` is an `ExceptT` monad and will always fail,
-then `it.filterMapM` will be finite even if `it` isn't. In the first case, consider
-using the `map`/`mapM`/`mapWithPostcondition` combinators instead, which provide more instances out of
-the box.
-
-If that does not help, the more general combinator `it.filterMapWithPostcondition f` makes it
-possible to manually prove `Finite` and `Productive` instances depending on the concrete choice of `f`.
+then `it.filterMapM` will be finite even if `it` isn't. In such cases, the termination proof needs
+to be done manually.
 
 **Performance:**
 
@@ -396,9 +392,9 @@ returned `Option` value.
 -/
 @[inline, expose]
 def IterM.filterMapM {α β γ : Type w} {m : Type w → Type w'} {n : Type w → Type w''}
-    [Iterator α m β] [Monad n] [MonadLiftT m n]
+    [Iterator α m β] [Monad n] [MonadAttach n] [MonadLiftT m n]
     (f : β → n (Option γ)) (it : IterM (α := α) m β) :=
-  (it.filterMapWithPostcondition (fun b => PostconditionT.lift (f b)) : IterM n γ)
+  (it.filterMapWithPostcondition (fun b => PostconditionT.attachLift (f b)) : IterM n γ)
 
 /--
 If `it` is an iterator, then `it.mapM f` is another iterator that applies a monadic
@@ -425,10 +421,8 @@ it.mapM     ---a'--b'--c'--d'-e'----⊥
 
 For certain mapping functions `f`, the resulting iterator will be finite (or productive) even though
 no `Finite` (or `Productive`) instance is provided. For example, if `f` is an `ExceptT` monad and
-will always fail, then `it.mapM` will be finite even if `it` isn't.
-
-If that does not help, the more general combinator `it.mapWithPostcondition f` makes it possible to
-manually prove `Finite` and `Productive` instances depending on the concrete choice of `f`.
+will always fail, then `it.mapM` will be finite even if `it` isn't. In such cases, the termination
+proof needs to be done manually.
 
 **Performance:**
 
@@ -436,8 +430,8 @@ For each value emitted by the base iterator `it`, this combinator calls `f`.
 -/
 @[inline, expose]
 def IterM.mapM {α β γ : Type w} {m : Type w → Type w'} {n : Type w → Type w''} [Iterator α m β]
-    [Monad n] [MonadLiftT m n] (f : β → n γ) (it : IterM (α := α) m β) :=
-  (it.mapWithPostcondition (fun b => PostconditionT.lift (f b)) : IterM n γ)
+    [Monad n] [MonadAttach n] [MonadLiftT m n] (f : β → n γ) (it : IterM (α := α) m β) :=
+  (it.mapWithPostcondition (fun b => PostconditionT.attachLift (f b)) : IterM n γ)
 
 /--
 If `it` is an iterator, then `it.filterM f` is another iterator that applies a monadic
@@ -465,10 +459,7 @@ it.filterM     ---a-----c-------⊥
 For certain mapping functions `f`, the resulting iterator will be finite (or productive) even though
 no `Finite` (or `Productive`) instance is provided. For example, if `f` is an `ExceptT` monad and
 will always fail, then `it.filterWithPostcondition` will be finite -- and productive -- even if `it`
-isn't.
-
-In such situations, the more general combinator `it.filterWithPostcondition f` makes it possible to
-manually prove `Finite` and `Productive` instances depending on the concrete choice of `f`.
+isn't. In such cases, the termination proof needs to be done manually.
 
 **Performance:**
 
@@ -476,9 +467,9 @@ For each value emitted by the base iterator `it`, this combinator calls `f`.
 -/
 @[inline, expose]
 def IterM.filterM {α β : Type w} {m : Type w → Type w'} {n : Type w → Type w''} [Iterator α m β]
-    [Monad n] [MonadLiftT m n] (f : β → n (ULift Bool)) (it : IterM (α := α) m β) :=
+    [Monad n] [MonadAttach n] [MonadLiftT m n] (f : β → n (ULift Bool)) (it : IterM (α := α) m β) :=
   (it.filterMapWithPostcondition
-    (fun b => (PostconditionT.lift (f b)).map (if ·.down = true then some b else none)) : IterM n β)
+    (fun b => (PostconditionT.attachLift (f b)).map (if ·.down = true then some b else none)) : IterM n β)
 
 /--
 If `it` is an iterator, then `it.filterMap f` is another iterator that applies a function `f` to all
