src/Init/Control/Lawful/MonadLift/Lemmas.lean
@@ -6,12 +6,21 @@ Authors: Quang Dao
 module
 
 prelude
+public import Init.Control.Id
 public import Init.Control.Lawful.Basic
 public import Init.Control.Lawful.MonadLift.Basic
 
 public section
 
 universe u v w
+
+theorem instMonadLiftTOfMonadLift_instMonadLiftTOfPure [Monad m] [Monad n] {_ : MonadLift m n}
+    [LawfulMonadLift m n] : instMonadLiftTOfMonadLift Id m n = Id.instMonadLiftTOfPure := by
+  have hext {a b : MonadLiftT Id n} (h : @a.monadLift = @b.monadLift) : a = b := by
+    cases a <;> cases b <;> simp_all
+  apply hext
+  ext α x
+  simp [monadLift, LawfulMonadLift.monadLift_pure]
 
 variable {m : Type u → Type v} {n : Type u → Type w} [Monad m] [Monad n] [MonadLiftT m n]
   [LawfulMonadLiftT m n] {α β : Type u}
